src/HOL/PreList.thy
@@ -8,12 +8,18 @@ header {* A Basis for Building the Theory of Lists *}
 
 theory PreList
 imports Presburger Relation_Power SAT Recdef Extraction Record
+uses "Tools/function_package/lexicographic_order.ML"
+     "Tools/function_package/fundef_datatype.ML"
 begin
 
 text {*
   This is defined separately to serve as a basis for
   theory ToyList in the documentation.
 *}
+
+(* The lexicographic_order method and the "fun" command *)
+setup LexicographicOrder.setup
+setup FundefDatatype.setup
 
 end
 
